coq/Syntax.v
@@ -13,12 +13,50 @@ Section TrustformerSyntax.
     Context (inputs_var: Type).
     Context (outputs_var: Type).
 
+    Inductive tf_unary_ops :=
+        | tf_not                                (* Bitwise NOT *)
+        (* | tf_sign_extend *)                        (* Sign extend *)
+        (* | tf_zero_extend_left *)                   (* Zero extend left *)
+        (* | tf_zero_extend_right *)                  (* Zero extend right *)
+        (* | tf_slice (offset: nat) (width: nat) *)   (* Slice *)
+        .
+
+    Inductive tf_comparison_ops :=
+        | tf_eq                                 (* Equal *)
+        | tf_neq                                (* Not equal *)
+        | tf_lt                                 (* Unsigned Less than *)
+        | tf_le                                 (* Unsigned Less than or equal *)
+        | tf_gt                                 (* Unsigned Greater than *)
+        | tf_ge                                 (* Unsigned Greater than or equal *)
+        .
+
+    Inductive tf_binary_ops :=
+        | tf_and                                (* Logical and *)
+        | tf_or                                 (* Logical or *)
+        | tf_xor                                (* Logical xor *)
+        | tf_add                                (* Addition *)
+        | tf_sub                                (* Subtraction *)
+        | tf_mul                                (* Multiplication *)
+        (* | tf_cmp (cmp_op: tf_comparison_ops)  *)   (* Comparison Operations *)
+        (* | tf_div *)
+        (* | tf_mod *)
+        .
+
+    Inductive tf_expr :=
+        | tf_const (value: nat)                                             (* Constant value *)
+        | tf_var (v: states_var)                                            (* Variable reference *) 
+        | tf_op1 (op: tf_unary_ops) (src: tf_expr)                       (* Unary operation *)
+        | tf_op2 (op: tf_binary_ops) (src1: tf_expr) (src2: tf_expr)  (* Binary operation *)
+        .
+
     (* Atomic operations on variables *)
     Inductive tf_ops :=
-        | tf_nop (* No operation *)
-        | tf_neg (x : states_var) (* Negate a variable *)
-        | tf_input (x : states_var) (y : inputs_var) (* Read input into variable *)
-        | tf_output (x : states_var) (y : outputs_var) (* Write variable to output *)
+        | tf_nop                                                (* No operation *)
+        | tf_assign (dst : states_var) (expr : tf_expr)         (* Unary Operations *)
+        
+        (* TODO: input & outputs should allow expressions instead of vars *)
+        | tf_input (dst : states_var) (src : inputs_var)        (* Read input into variable *)
+        | tf_output (dst : outputs_var) (src : states_var)      (* Write variable to output *)
         . 
 
 End TrustformerSyntax.
